src/Init/Data/UInt/BasicAux.lean
@@ -220,7 +220,7 @@ instance UInt32.instOfNat : OfNat UInt32 n := ⟨UInt32.ofNat n⟩
 
 theorem UInt32.ofNatLT_lt_of_lt {n m : Nat} (h1 : n < UInt32.size) (h2 : m < UInt32.size) :
      n < m → UInt32.ofNatLT n h1 < UInt32.ofNat m := by
-  simp only [(· < ·), BitVec.toNat, ofNatLT, BitVec.ofNatLT, ofNat, BitVec.ofNat, Fin.ofNat',
+  simp only [(· < ·), BitVec.toNat, ofNatLT, BitVec.ofNatLT, ofNat, BitVec.ofNat, Fin.ofNat,
     Nat.mod_eq_of_lt h2, imp_self]
 
 @[deprecated UInt32.ofNatLT_lt_of_lt (since := "2025-02-13")]
@@ -229,7 +229,7 @@ theorem UInt32.ofNat'_lt_of_lt {n m : Nat} (h1 : n < UInt32.size) (h2 : m < UInt
 
 theorem UInt32.lt_ofNatLT_of_lt {n m : Nat} (h1 : n < UInt32.size) (h2 : m < UInt32.size) :
      m < n → UInt32.ofNat m < UInt32.ofNatLT n h1 := by
-  simp only [(· < ·), BitVec.toNat, ofNatLT, BitVec.ofNatLT, ofNat, BitVec.ofNat, Fin.ofNat',
+  simp only [(· < ·), BitVec.toNat, ofNatLT, BitVec.ofNatLT, ofNat, BitVec.ofNat, Fin.ofNat,
     Nat.mod_eq_of_lt h2, imp_self]
 
 @[deprecated UInt32.lt_ofNatLT_of_lt (since := "2025-02-13")]
