src/Init/Grind/CommRing/Fin.lean
@@ -15,20 +15,20 @@ namespace Lean.Grind
 namespace Fin
 
 instance (n : Nat) [NeZero n] : NatCast (Fin n) where
-  natCast a := Fin.ofNat' n a
+  natCast a := Fin.ofNat n a
 
 @[expose]
 def intCast [NeZero n] (a : Int) : Fin n :=
   if 0 ≤ a then
-    Fin.ofNat' n a.natAbs
+    Fin.ofNat n a.natAbs
   else
-    - Fin.ofNat' n a.natAbs
+    - Fin.ofNat n a.natAbs
 
 instance (n : Nat) [NeZero n] : IntCast (Fin n) where
   intCast := Fin.intCast
 
 theorem intCast_def {n : Nat} [NeZero n] (x : Int) :
-    (x : Fin n) = if 0 ≤ x then Fin.ofNat' n x.natAbs else -Fin.ofNat' n x.natAbs := rfl
+    (x : Fin n) = if 0 ≤ x then Fin.ofNat n x.natAbs else -Fin.ofNat n x.natAbs := rfl
 
 -- TODO: we should replace this at runtime with either repeated squaring,
 -- or a GMP accelerated function.
@@ -72,7 +72,7 @@ theorem left_distrib (a b c : Fin n) : a * (b + c) = a * b + a * c := by
   cases a; cases b; cases c; simp [Fin.mul_def, Fin.add_def, Nat.left_distrib]
 
 theorem ofNat_succ [NeZero n] (a : Nat) : OfNat.ofNat (α := Fin n) (a+1) = OfNat.ofNat a + 1 := by
-  simp [OfNat.ofNat, Fin.add_def, Fin.ofNat']
+  simp [OfNat.ofNat, Fin.add_def, Fin.ofNat]
 
 theorem sub_eq_add_neg [NeZero n] (a b : Fin n) : a - b = a + -b := by
   cases a; cases b; simp [Fin.neg_def, Fin.sub_def, Fin.add_def, Nat.add_comm]
@@ -107,8 +107,8 @@ instance (n : Nat) [NeZero n] : CommRing (Fin n) where
 
 instance (n : Nat) [NeZero n] : IsCharP (Fin n) n where
   ofNat_eq_zero_iff x := by
-    change Fin.ofNat' _ _ = Fin.ofNat' _ _ ↔ _
-    simp only [Fin.ofNat']
+    change Fin.ofNat _ _ = Fin.ofNat _ _ ↔ _
+    simp only [Fin.ofNat]
     simp only [Nat.zero_mod]
     simp only [Fin.mk.injEq]
 
